Update dynamic frames idiom (#972)
* Change fresh(Repr - {this} ...) to fresh(Repr ...)

* For autocontracts, generate constructor postcondition "fresh(Repr)", not "fresh(Repr - {this})"

* Add postcondition "Valid() ==> this in Repr" to Valid() for :autocontracts

* Add "Valid() ==> this in Repr" as postcondition of Valid() (in most substantial test cases)

Test/VSComp2010/Problem3-FindZero.dfy
@@ -28,8 +28,9 @@ class Node {
   var head: int
   var next: Node?
 
-  function Valid(): bool
+  predicate Valid()
     reads this, Repr
+    ensures Valid() ==> this in Repr
   {
     this in Repr &&
     1 <= |List| && List[0] == head &&
